theories/rules/ldr.v
@@ -38,10 +38,10 @@ Proof.
   iDestruct "Hσ" as "(Hσtok & Hmem & Hreg & Htxown & Hrx1 & Hrx2 & Hown & Haccess & Hrest)".
   pose proof (decode_instruction_valid w1 instr Hdecode) as Hvalidinstr.
   rewrite Hinstr in Hvalidinstr.
-  inversion Hvalidinstr as [| | src dst H3' H4' Hneqrarb | | | | |]; subst src dst; clear Hvalidinstr.
+  inversion Hvalidinstr as [| | src dst H3' H4' Hneqrarb | | | | | | |]; subst src dst; clear Hvalidinstr.
   destruct H3' as [HneqPCa HneqNZa].
   destruct H4' as [HneqPCb HneqNZb].
-  iDestruct ((gen_reg_valid3 i PC ai ra w3 rb a Hcur HneqPCa HneqPCb Hneqrarb) with "Hreg Hpc Hra Hrb") as "[%HPC [%Hra %Hrb]]".
+  iDestruct ((gen_reg_valid3 i PC ai ra w3 rb a Hcur) with "Hreg Hpc Hra Hrb") as "[%HPC [%Hra %Hrb]]".
   (* valid pt *)
   assert (Hais : to_pid_aligned ai ∈ s). set_solver.
   assert (Has : to_pid_aligned a ∈ s). set_solver.
@@ -109,10 +109,10 @@ Proof.
   iDestruct "Hσ" as "(Htok & Hmem & Hreg & Htxown & Hrx1 & Hrx2 & Hown & Haccess & Hrest)".
   pose proof (decode_instruction_valid w1 instr Hdecode) as Hvalidinstr.
   rewrite Hinstr in Hvalidinstr.
-  inversion Hvalidinstr as [| | src dst H3' H4' Hneqrarb | | | | |]; subst src dst; clear Hvalidinstr.
+  inversion Hvalidinstr as [| | src dst H3' H4' Hneqrarb | | | | | | |]; subst src dst; clear Hvalidinstr.
   destruct H3' as [HneqPCa HneqNZa].
   destruct H4' as [HneqPCb HneqNZb].
-  iDestruct ((gen_reg_valid3 i PC ai ra w3 rb a Hcur HneqPCa HneqPCb Hneqrarb) with "Hreg Hpc Hra Hrb") as "[%HPC [%Hra %Hrb]]".
+  iDestruct ((gen_reg_valid3 i PC ai ra w3 rb a Hcur) with "Hreg Hpc Hra Hrb") as "[%HPC [%Hra %Hrb]]".
   iDestruct ((gen_mem_valid ai w1) with "Hmem Hapc") as "%Hpc".
   iDestruct ((gen_access_valid_addr_elem ai s Hais) with "Haccess Hacc") as "%Hai".
   iDestruct (gen_tx_valid i p with "Htx Htxown") as %Htx.
