theories/rules/str.v
@@ -38,12 +38,12 @@ Proof.
   iDestruct "Hσ" as "(Htok & Hmem & Hreg & Htx & Hrxpage & Hrx2 & Hown & Haccess & Hrest)".
   pose proof (decode_instruction_valid w1 instr Hdecode) as Hvalidinstr.
   rewrite Hinstr in Hvalidinstr.
-  inversion Hvalidinstr as [ | | | src dst Hvalidra Hvalidrb Hneqrarb | | | |] .
+  inversion Hvalidinstr as [ | | | src dst Hvalidra Hvalidrb Hneqrarb | | | | | |] .
   subst src dst.
   inversion Hvalidra as [ HneqPCa HneqNZa ].
   inversion Hvalidrb as [ HneqPCb HneqNZb ].
   (* valid regs *)
-  iDestruct ((gen_reg_valid3 i PC ai ra w2 rb a Hcur HneqPCa HneqPCb Hneqrarb ) with "Hreg Hpc Hra Hrb") as "[%HPC [%Hra %Hrb]]".
+  iDestruct ((gen_reg_valid3 i PC ai ra w2 rb a Hcur) with "Hreg Hpc Hra Hrb") as "[%HPC [%Hra %Hrb]]".
   (* valid pt *)
   assert (Hais : to_pid_aligned ai ∈ s). set_solver.
   assert (Has : to_pid_aligned a ∈ s). set_solver.
@@ -110,10 +110,10 @@ Proof.
   iDestruct "Hσ" as "(Htok & Hmem & Hreg & Htx & Hrxown & Hrx2 & Hown & Haccess & Hrest)".
   pose proof (decode_instruction_valid w1 instr Hdecode) as Hvalidinstr.
   rewrite Hinstr in Hvalidinstr.
-  inversion Hvalidinstr as [| | | src dst H3' H4' Hneqrarb | | | |]; subst src dst; clear Hvalidinstr.
+  inversion Hvalidinstr as [| | | src dst H3' H4' Hneqrarb | | | | | |]; subst src dst; clear Hvalidinstr.
   destruct H3' as [HneqPCa HneqNZa].
   destruct H4' as [HneqPCb HneqNZb].
-  iDestruct ((gen_reg_valid3 i PC ai ra w2 rb a Hcur HneqPCa HneqPCb Hneqrarb) with "Hreg Hpc Hra Hrb") as "[%HPC [%Hra %Hrb]]".
+  iDestruct ((gen_reg_valid3 i PC ai ra w2 rb a Hcur) with "Hreg Hpc Hra Hrb") as "[%HPC [%Hra %Hrb]]".
   iDestruct ((gen_mem_valid ai w1) with "Hmem Hapc") as "%Hpc".
   iDestruct ((gen_access_valid_addr_elem ai s Hais) with "Haccess Hacc") as "%Hai".
   iDestruct (gen_rx_pid_valid i p with "Hrx Hrxown") as %Hrx.
